\begin{frame}{Lagrange Interpolation Operators}
    \textbf{The Lagrange interpolation operator:}
    \begin{equation*}
        \mathcal{I}_h^m(f)(x)=\sum_{i=1}^m f\left(x_i\right) P_i(x)
    \end{equation*} 
    with $P_i\left(x_j\right)=\delta_{i j}$


    \textbf{The Deep Lagrange Interpolation:}
    \begin{equation*}
        \mathcal{I}_d^m(f)=\sum_{i=1}^n \frac{f\left(x_i\right)}{u_\theta\left(x_i\right)} P_i(x) u_\theta(x)=\mathcal{I}^m\left(\frac{f}{u_\theta}\right) u_\theta(x)
    \end{equation*}

    With $P_i\left(x_j\right)=\delta_{i j}$
    Using this choice, we obtain that $\mathcal{I}_d(f)\left(x_i\right)=f\left(x_i\right)$ as the classical interpolator.
    

    % \textbf{ $u_{\theta i}$ Function:}

    % \begin{equation*}
    %     u_{\theta_i}(x)= u_0(x + \epsilon -at)

    % \end{equation*}
\end{frame}
